theories/itree.v
@@ -1,0 +1,383 @@
+From ITree Require Export ITree ITreeFacts.
+From ITree Require Export ITree.
+Require Export refframe.module.
+Require Import refframe.trefines.
+
+Notation "' x ← y ;;; z" := (ITree.bind y (λ x : _, z))
+  (at level 20, x pattern, y at level 100, z at level 200) : stdpp_scope.
+Notation "x ← y ;;; z" := (ITree.bind y (λ x : _, z))
+  (at level 20, y at level 100, z at level 200) : stdpp_scope.
+Notation "y ;;;; z" := (ITree.bind y (λ _, z))
+  (at level 100, z at level 200, right associativity) : stdpp_scope.
+
+
+Inductive moduleE (EV S : Type) : Type → Type :=
+| IVis (e : EV) : moduleE EV S unit
+| IAll (T : Type) : moduleE EV S T
+| IExist (T : Type) : moduleE EV S T
+| IGet : moduleE EV S S
+| IPut (s : S) : moduleE EV S unit
+.
+Arguments IVis {_ _}.
+Arguments IAll {_ _}.
+Arguments IExist {_ _}.
+Arguments IGet {_ _}.
+Arguments IPut {_ _}.
+
+Inductive mod_itree_step EV S : (itree (moduleE EV S) unit * S) → option EV → ((itree (moduleE EV S) unit * S) → Prop) → Prop :=
+| ITauS t t' s:
+  observe t = TauF t' →
+  mod_itree_step EV S (t, s) None (λ σ', σ' = (t', s))
+| IVisS t t' s e:
+  observe t = VisF (IVis e) t' →
+  mod_itree_step EV S (t, s) (Some e) (λ σ', σ' = (t' tt, s))
+.
+
+Definition mod_itree EV S := Mod (mod_itree_step EV S).
+Inductive under_tall {EV} : trace EV → (trace EV → Prop) → Prop :=
+| UTEnd κs (P : _ → Prop):
+  P κs →
+  under_tall κs P
+| UTAll T f κs (P : _ → Prop):
+  (∀ x, under_tall (f x) P) →
+  tall T f ⊆ κs →
+  under_tall κs P.
+
+Lemma under_tall_mono {EV} (κs1 κs2 : trace EV) (P1 P2 : _ → Prop):
+  under_tall κs1 P1 →
+  κs1 ⊆ κs2 →
+  (∀ κs1' κs2', κs1' ⊆ κs2' → P1 κs1' → P2 κs2') →
+  under_tall κs2 P2.
+Proof.
+  move => Hall. elim: Hall κs2.
+  - move => ????? HP. econs. apply: HP; [..|done] => //.
+  - move => ????? IH ??? HP. apply: UTAll; [|by etrans]. move => ?. apply: IH; [done|].
+    done.
+Qed.
+
+Global Instance under_tall_proper {EV} :
+  Proper ((⊆) ==> ((⊆) ==> impl) ==> impl) (@under_tall EV).
+Proof. move => κs1 κs2 Hsub ?? HP Hall. by apply: under_tall_mono. Qed.
+
+Lemma thas_trace_under_tall {EV} m (κs1 κs2 : trace EV) (P1 Pσ : _ → Prop) σ:
+  under_tall κs1 P1 →
+  κs1 ⊆ κs2 →
+  (∀ κs', P1 κs' → σ ~{ m, κs' }~>ₜ Pσ) →
+  σ ~{ m, κs2 }~>ₜ Pσ.
+Proof.
+  move => Hall. elim: Hall κs2.
+  - move => ???? <- HP. by apply: HP.
+  - move => ????? IH Hκ ?? HP. apply: TTraceAll; [|by etrans]. naive_solver.
+Qed.
+
+Lemma tnhas_trace_under_tall {EV} m (κs1 κs2 : trace EV) (P1 Pσ : _ → Prop) σ n:
+  under_tall κs1 P1 →
+  κs1 ⊆ κs2 →
+  (∀ κs', P1 κs' → σ ~{ m, κs', n }~>ₜ Pσ) →
+  σ ~{ m, κs2, n }~>ₜ Pσ.
+Proof.
+  move => Hall. elim: Hall κs2.
+  - move => ???? <- HP. by apply: HP.
+  - move => ????? IH Hκ ?? HP. apply: TNTraceAll; [|by etrans |]. naive_solver. done.
+Qed.
+
+Lemma thas_trace_inv' {EV} (m : module EV) κs (Pσ : _ → Prop) σ:
+  σ ~{ m, κs }~>ₜ Pσ →
+  under_tall κs (λ κs, (tnil ⊆ κs ∧ Pσ σ) ∨
+    ∃ κ κs' Pσ2, m_step m σ κ Pσ2 ∧ (∀ σ2, Pσ2 σ2 → σ2 ~{ m, κs' }~>ₜ Pσ) ∧ tapp (option_trace κ) κs' ⊆ κs).
+Proof.
+  elim.
+  - move => ?????. econs. naive_solver.
+  - move => *. econs. naive_solver.
+  - move => ?????? IH ?. apply: UTAll; [|done]. done.
+Qed.
+
+Lemma tnhas_trace_inv' {EV} (m : module EV) κs (Pσ : _ → Prop) σ n:
+  σ ~{ m, κs, n }~>ₜ Pσ →
+  under_tall κs (λ κs, (tnil ⊆ κs ∧ Pσ σ) ∨
+    ∃ κ κs' Pσ2 fn, m_step m σ κ Pσ2 ∧ (∀ σ2 (H : Pσ2 σ2), σ2 ~{ m, κs', fn (σ2 ↾ H) }~>ₜ Pσ)
+      ∧ tapp (option_trace κ) κs' ⊆ κs ∧ (∀ x, fn x ⊂ n)).
+Proof.
+  elim.
+  - move => ??????. econs. naive_solver.
+  - move => *. econs. right. naive_solver.
+  - move => ???????? IH ??. apply: UTAll; [|done].
+    move => ?. apply: under_tall_mono; [done..|].
+    move => ?? Hκ [[??]|?]; [left|right].
+    + split; [|done]. by rewrite -Hκ.
+    + destruct_all?. eexists _, _, _, _. split_and! => //. { by etrans. } move => ?.
+      by apply: ti_lt_le.
+Qed.
+
+Lemma tnhas_trace_Tau' {EV S} t t' n n' Pσ s κs:
+  observe t = TauF t' →
+  (t', s) ~{mod_itree EV S, κs, n}~>ₜ Pσ →
+  n ⊂ n' →
+  (t, s) ~{mod_itree EV S, κs, n'}~>ₜ Pσ.
+Proof.
+  move => Htau Ht Hsub. apply: (TNTraceStep _ _ (λ _, n)); [by econs| |done|simpl; done] => /= ? ->. done.
+Qed.
+
+Lemma thas_trace_Tau' {EV S} t t' Pσ s κs:
+  observe t = TauF t' →
+  (t', s) ~{mod_itree EV S, κs}~>ₜ Pσ →
+  (t, s) ~{mod_itree EV S, κs}~>ₜ Pσ.
+Proof. move => Htau Ht. tstep_None; [by econs|]. naive_solver. Qed.
+
+Lemma tnhas_trace_Tau_inv' {EV S} t t' n Pσ s κs:
+  observe t' = TauF t →
+  (t', s) ~{mod_itree EV S, κs, n}~>ₜ Pσ →
+  under_tall κs (λ κs, (tnil ⊆ κs ∧ Pσ (t', s)) ∨
+    ∃ n', n' ⊂ n ∧ (t, s) ~{ mod_itree _ _,  κs, n' }~>ₜ Pσ).
+Proof.
+  move => Htau /tnhas_trace_inv' Ht. apply: under_tall_mono; [done..|] => {Ht} κs1 κs2 /= Hκs1 [[??]|?].
+  { left. split; [by etrans|done]. }
+  right. destruct_all!. invert_all @mod_itree_step; rewrite ->Htau in *; simplify_eq.
+  eexists _. split; [done|]. rewrite -Hκs1 -H0. naive_solver.
+  Unshelve. done.
+Qed.
+
+(*
+Lemma tnhas_trace_Tau_inv' {EV S} t t' n Pσ s κs:
+  observe t' = TauF t →
+  (t', s) ~{mod_itree EV S, κs, n}~>ₜ Pσ →
+  (* (tnil ⊆ κs ∧ Pσ (t', s)) ∨ ∃ n', n' ⊂ n ∧ (t, s) ~{mod_itree EV S, κs, n'}~>ₜ Pσ *)
+  ∃ n', n' ⊂ n ∧ (t, s) ~{mod_itree EV S, κs, n'}~>ₜ Pσ.
+  (* (t, s) ~{mod_itree EV S, tnil, tiO}~>ₜ (λ σ, σ = (t, s) ∧ *)
+      (* ((tnil ⊆ κs ∧ Pσ (t', s)) ∨ ). *)
+Proof.
+  move => Htau. move Hσ: (t, s) => σ. move Hσ': (t', s) => σ' Ht.
+  elim: Ht t t' Hσ Hσ' Htau; clear.
+  - admit.
+    (* tend. naive_solver. *)
+  - move => ?????????? IH ? Hκs ???? Htau. simplify_eq. invert_all @m_step; rewrite ->Htau in *; simplify_eq.
+  (* tend. split; [done|]. right. eexists _. split. 2: { rewrite -Hκs. done. } done. *)
+    admit.
+  - move => ???????? IH Hκs??????. subst.
+    (* apply: TNTraceAll; [|done|done] => ?. by apply: IH. *)
+Abort.
+
+Lemma tnhas_trace_Tau_inv' {EV S} t t' n Pσ Pσ' s κs:
+  (prod_relation (eutt eq) (=) ==> iff)%signature Pσ Pσ' →
+  observe t' = TauF t →
+  (t', s) ~{mod_itree EV S, κs, n}~>ₜ Pσ →
+  (t, s) ~{mod_itree EV S, κs, n}~>ₜ Pσ'.
+Proof.
+  move => Hproper Htau. move Hσ: (t, s) => σ. move Hσ': (t', s) => σ' Ht.
+  elim: Ht t t' Hσ Hσ' Hproper Htau; clear.
+  - move => ?????? t t' ?? Hproper Htau. tend. subst. eapply Hproper; [|done]. split => //=.
+    by rewrite (itree_eta t') Htau tau_eutt.
+  - move => ?????????? IH ? Hκs ???? Hproper Htau. simplify_eq.
+    invert_all @m_step; rewrite ->Htau in *; simplify_eq.
+    apply: tnhas_trace_mono; [done|done| | ].
+    + by apply ti_lt_impl_le.
+    + move => ??. eapply Hproper; [|done]. done.
+  - move => ???????? IH Hκs???????. subst.
+    apply: TNTraceAll; [|done|done] => ?. by apply: IH.
+  Unshelve. done.
+Qed.
+ *)
+
+Lemma thas_trace_Tau_inv' {EV S} t t' Pσ Pσ' s κs:
+  (prod_relation (eutt eq) (=) ==> iff)%signature Pσ Pσ' →
+  observe t' = TauF t →
+  (t', s) ~{mod_itree EV S, κs}~>ₜ Pσ →
+  (t, s) ~{mod_itree EV S, κs}~>ₜ Pσ'.
+Proof.
+  move => Hproper Htau /thas_trace_n[??].
+  apply thas_trace_n. eexists _.
+  (* by apply: tnhas_trace_Tau_inv'. *)
+(* Qed. *)
+Admitted.
+
+Lemma tnhas_trace_inv {EV} (m : module EV) σ (Pσ : _ → Prop) (P : _ → _ → Prop):
+  (∀ n, Pσ σ → P n tnil) →
+  (∀ κ κs' Pσ2 n f,
+      m.(m_step) σ κ Pσ2 →
+      (∀ σ2 (H:Pσ2 σ2), σ2 ~{ m, κs', f (σ2 ↾ H) }~>ₜ Pσ) →
+      (∀ x, f x ⊂ n) →
+      P n (tapp (option_trace κ) κs')) →
+  (∀ T f fn n, (∀ x, P (fn x) (f x)) → (∀ x, fn x ⊆ n) → P n (tall T f)) →
+  (∀ n κs κs', P n κs' → κs' ⊆ κs → P n κs) →
+  ∀ n κs, σ ~{ m, κs, n }~>ₜ Pσ → P n κs.
+Proof.
+  move => HEnd HStep Hall Hsub κs n Ht.
+  elim: Ht HEnd HStep Hall Hsub; clear.
+  - naive_solver.
+  - naive_solver.
+  - move => T f fn n σ κs Pσ ? IH ?? HEnd HStep Hall Hsub.
+    apply: (Hsub); [|done].
+    apply: (Hall) => ? //.
+    apply: IH; naive_solver.
+Qed.
+Ltac tnhas_trace_inv H :=
+  lazymatch type of H with
+  | _ ~{ _, ?κs, ?n }~>ₜ _ => pattern n; pattern κs
+  end;
+  lazymatch goal with
+  | |- (λ κs', (λ n', @?P n' κs') ?n) ?κs => change (P n κs)
+  end;
+  apply: (tnhas_trace_inv _ _ _ _ _ _ _ _ _ _ H); try clear H; [ | |
+     try by [move => *; apply subtrace_all_r; eauto];
+     try by [move => *; apply thas_trace_all; eauto] |
+     try by [move => ???? <-]
+ ].
+
+
+Lemma tnhas_trace_Ret_inv' {EV S} t x n Pσ s κs:
+  observe t = RetF x →
+  (t, s) ~{mod_itree EV S, κs, n}~>ₜ Pσ →
+  under_tall κs (λ κs, tnil ⊆ κs ∧ Pσ (t, s)).
+Proof.
+  move => Hret /tnhas_trace_inv' Ht.
+  apply: under_tall_mono; [done..|] => {Ht} κs1 κs2 /= Hκs [[??]|]. { split => //. by rewrite -Hκs. }
+  move => ?. destruct_all!. invert_all @mod_itree_step; rewrite ->Hret in *; simplify_eq.
+Qed.
+(*
+Lemma thas_trace_Tau' {EV S} t t' Pσ s κs:
+  observe t = TauF t' →
+  (t', s) ~{mod_itree EV S, κs}~>ₜ Pσ →
+  (t, s) ~{mod_itree EV S, κs}~>ₜ Pσ.
+Proof. move => Htau Ht. tstep_None; [by econs|]. naive_solver. Qed.
+*)
+From Paco Require Import paco.
+
+Lemma thas_trace_eutt_mono {EV S} t t' s κs Pσ Pσ':
+  (prod_relation (eutt eq) (=) ==> iff)%signature Pσ Pσ' →
+  (t, s) ~{ mod_itree EV S, κs }~>ₜ Pσ →
+  t ≈ t' →
+  (t', s) ~{ mod_itree EV S, κs }~>ₜ Pσ'.
+Proof.
+  move => HP /thas_trace_n[n Ht] Heq.
+  elim/(well_founded_ind ti_lt_wf): n κs t t' s Ht Heq HP.
+  move => n IHn κs t t' s Ht Heq HP.
+  punfold Heq. unfold eqit_ in Heq at 1.
+  move: Heq. move Hot: (observe t) => ot. move Hot': (observe t') => ot' Heq.
+  elim: Heq t t' n IHn Ht Hot Hot'.
+  - move => ?? -> t t' n IHn Ht Hot Hot'.
+    move: Ht => /(tnhas_trace_Ret_inv' _ _ _ _ _)Ht. specialize (Ht _ ltac:(done)).
+    apply: thas_trace_under_tall; [done..|] => ? [??]. tend.
+    eapply HP; [|done]. split; [|done] => /=. rewrite (itree_eta t) Hot (itree_eta t') Hot'. done.
+  - move => m1 m2 [REL|//] t t' n IHn Ht Hot Hot'. rewrite -/(eqit _ _ _) in REL.
+    apply: thas_trace_Tau'; [done|]. revert IHn.
+    tnhas_trace_inv Ht. { tend. eapply HP; [|done]. split => //=. by rewrite (itree_eta t) Hot tau_eutt REL. }
+    2: { move => ???? IH ? IHn. apply thas_trace_all => ?. apply: IH => *. apply: IHn => //. by apply: ti_lt_le. }
+    move => ?????? Ht Hlt IHn. invert_all @m_step; rewrite -> Hot in *; simplify_eq.
+    specialize (Ht _ ltac:(done)).
+    apply: IHn; [done|done| |done]. by rewrite REL.
+  - admit.
+  - move => t1 ot2 ? REL IH t t' n IHn Ht Hot Hot'.
+    move: Ht => /(tnhas_trace_Tau_inv' _ _ _ _ _ _)Ht. specialize (Ht _ _ ltac:(done) ltac:(done)).
+    apply: IH => //. apply: tnhas_trace_mono; [done..|] => ??. eapply HP; [|done]. done.
+  - move => ot1 t2 ? REL IH t t' n IHn Ht Hot Hot'.
+    tstep_None; [by econs|] => ? ->. by apply: IH.
+    Unshelve.
+Admitted.
+
+Global Instance mod_itree_proper EV S b1 b2:
+  Proper ((prod_relation (eqit eq b1 b2) (=)) ==> (=) ==> (prod_relation (eutt eq) (=) ==> iff) ==> iff) (thas_trace (mod_itree EV S)).
+Proof.
+  move => [??] [??] [/= Heq ->] ?? -> ?? Hf.
+  split => ?.
+  all: apply: thas_trace_eutt_mono; [try done| done |].
+  - by apply: eqit_mon; [| | |done].
+  - move => ?? [??]. symmetry. by apply Hf.
+  - symmetry. by apply: eqit_mon; [| | |done].
+Qed.
+
+(*
+(* TODO: add step index to thas_trace and make sure that this step
+index only goes down in calls to sim *)
+Lemma thas_trace_eqitF' {EV S} t t' s κs Pσ b1 b2 sim :
+  (go t, s) ~{ mod_itree EV S, κs }~>ₜ Pσ →
+  eqitF eq b1 b2 id sim t t' →
+  (∀ m1 m2 κs, (m1, s) ~{ mod_itree EV S, κs }~>ₜ Pσ → sim m1 m2 → (m2, s) ~{ mod_itree EV S, κs }~>ₜ Pσ) →
+  (∀ t1 t2 s, Pσ (t1, s) → t1 ≈ t2 → Pσ (t2, s)) →
+  (go t', s)  ~{ mod_itree EV S, κs }~>ₜ Pσ.
+Proof.
+  move => Ht Heq Hsim HRR.
+  induction Heq.
+  - thas_trace_inv Ht. subst. 2: intros; invert_all @m_step. tend.
+  - tstep_None; [by constructor|] => ? ->. apply: Hsim; [|done].
+    thas_trace_inv Ht. { tend. apply: HRR; [done|]. by rewrite tau_eutt. }
+    move => ?????. invert_all @m_step. done.
+  - thas_trace_inv Ht. { tend. apply: HRR; [done|]. admit. }
+    move => ???? IH. invert_all' @m_step; simplify_eq.
+    + simpl in H3; simplify_eq; simplify_K.
+      apply: Hsim.
+      * tstep; [ | |done].
+        admit.
+      * tstep; [ | |done].
+        admit.
+        (* => /= ??. apply: IH. *)
+      apply UIPM.inj_pair2 in H2.
+  - apply IHHeq. admit.
+  - admit.
+Admitted.
+
+Lemma thas_trace_eutt_mono'' {EV S} t t' s κs Pσ :
+  (go t, s) ~{ mod_itree EV S, κs }~>ₜ Pσ →
+  go t ≈ go t' →
+  (∀ t1 t2 s, Pσ (t1, s) → t1 ≈ t2 → Pσ (t2, s)) →
+  (go t', s) ~{ mod_itree EV S, κs }~>ₜ Pσ.
+Proof.
+  move => Ht Heq Hproper. punfold Heq.
+  apply: thas_trace_eqitF'; [done|done| |].
+  - move => ??? [Heq2 | //].
+
+  Lemma thas_trace_eutt_mono' {EV S} σ1 σ2 κs Pσ :
+  σ1 ~{ mod_itree EV S, κs }~>ₜ Pσ →
+  σ1.1 ≈ σ2.1 →
+  σ1.2 = σ2.2 →
+  (∀ t1 t2 s, Pσ (t1, s) → t1 ≈ t2 → Pσ (t2, s)) →
+  σ2 ~{ mod_itree EV S, κs }~>ₜ Pσ.
+Proof.
+  move => Ht Heq1 Heq2 Hproper.
+  destruct σ1 as [t s], σ2 as [t' s']. simplify_eq/=. punfold Heq1.
+
+  apply thas_trace_eqitF'.
+  induction Heq1; simplify_eq.
+  elim: Heq1.
+
+  elim: Ht σ2 Heq1 Heq2 Hproper.
+  - move => [??] ???? [??] /= ??. subst. tend. naive_solver.
+  - move => [t1 ?] ??????? IH Hκs [??]/= Heq ??. subst. rewrite -Hκs. invert_all @m_step.
+    + apply IH => /=; [|done..]. rewrite -Heq (itree_eta t1) H3. rewrite tau_eutt. done.
+    + tstep_Some.
+      * apply IVisS.
+  - move => ?????? IH Hκs ????. rewrite -Hκs. apply thas_trace_all => ?. by apply IH.
+Qed.
+
+Lemma thas_trace_eutt_mono {EV S} t t' s κs Pσ :
+  (t, s) ~{ mod_itree EV S, κs }~>ₜ Pσ →
+  t ≈ t' →
+  (∀ t1 t2 s, Pσ (t1, s) → t1 ≈ t2 → Pσ (t2, s)) →
+  (t', s) ~{ mod_itree EV S, κs }~>ₜ Pσ.
+Proof. move => ???. by apply: thas_trace_eutt_mono'. Qed.
+*)
+
+Require refframe.example_modules.
+Module itree_examples.
+Import refframe.example_modules.
+
+Lemma itree_trefines_tau_l :
+  trefines (MS (mod_itree nat unit) (Tau (Ret tt), tt)) (MS (mod_itree nat unit) (Ret tt, tt)).
+Proof. constructor => /= ?. rewrite tau_eutt. done. Qed.
+
+Lemma mod1_trefines_itree :
+  trefines (MS mod1 0) (MS (mod_itree nat unit) ((_ ← trigger (IVis 1) ;;; Ret tt), tt)).
+Proof.
+  constructor => /= ? Ht.
+  thas_trace_inv Ht; [tend|] => ???? Ht. invert_all @m_step.
+  rewrite bind_trigger.
+  tstep_Some; [by econs|] => ? ->.
+  thas_trace_inv Ht; [tend|] => ???? Ht. invert_all @m_step.
+Qed.
+
+Lemma itree_trefines_mod1 :
+  trefines (MS (mod_itree nat unit) ((trigger (IVis 1);;;; Ret tt), tt)) (MS mod1 0).
+Proof.
+  constructor => /= ?. rewrite bind_trigger.
+Abort.
+
+End itree_examples.
