theories/trace_index.v
@@ -1,0 +1,103 @@
+Require Import refframe.base.
+Require Import refframe.axioms.
+
+Inductive trace_index : Type :=
+| tiO | tiS (n : trace_index) | tiChoice (T : Type) (f : T → trace_index).
+
+Inductive ti_le : trace_index → trace_index → Prop :=
+| ti_le_O n : ti_le tiO n
+| ti_le_S_S n1 n2 : ti_le n1 n2 → ti_le (tiS n1) (tiS n2)
+(* | ti_le_choice_r T f n : (∀ x, ti_le n (f x)) → ti_le n (tiChoice T f) *)
+(* | ti_le_choice_l T f n x : ti_le (f x) n → ti_le (tiChoice T f) n *)
+| ti_le_choice_l T f n : (∀ x, ti_le (f x) n) → ti_le (tiChoice T f) n
+| ti_le_choice_r T f n x : ti_le n (f x) → ti_le n (tiChoice T f)
+.
+Global Instance ti_le_subseteq : SubsetEq trace_index := ti_le.
+Global Instance ti_le_rewrite : RewriteRelation (ti_le) := {}.
+Global Instance ti_le_equiv : Equiv trace_index := λ n1 n2, ti_le n1 n2 ∧ ti_le n2 n1.
+
+Global Instance ti_le_preorder : PreOrder (⊆@{trace_index}).
+Proof.
+  constructor.
+  - move => n. elim: n.
+    + constructor.
+    + by constructor.
+    + econs => ?. econs. naive_solver.
+  - move => x y z Hx. elim: Hx z.
+    + constructor.
+    + move => ????. elim.
+      * inversion 1.
+      * move => ? IH Hs. inversion_clear Hs; simplify_eq. constructor. naive_solver.
+      * move => ?? IH Hs. inversion Hs; simplify_K. econs. naive_solver.
+    + move => ???????. econs. naive_solver.
+    + move => ??????. elim.
+      * inversion 1; simplify_K. naive_solver.
+      * move => ? IH Hs. inversion Hs; simplify_K. naive_solver.
+      * move => ?? IH Hs. inversion Hs; simplify_K.
+        -- naive_solver.
+        -- econs. naive_solver.
+Qed.
+Global Instance ti_equiv_equiv : Equivalence (≡@{trace_index}).
+Proof.
+  constructor.
+  - done.
+  - move => ?? [??]. done.
+  - move => ??? [??] [??]. by split; etrans.
+Qed.
+
+Lemma ti_lt_impl_le (n1 n2 : trace_index):
+  n1 ⊂ n2 →
+  n1 ⊆ n2.
+Proof. move => [??]. done. Qed.
+
+Lemma ti_le_S n:
+  n ⊆ tiS n.
+Proof.
+  elim: n.
+  - econs.
+  - by econs.
+  - move => ?? IH. constructor => ?. etrans; [apply: IH|]. econs. by econs.
+Qed.
+
+Lemma ti_not_le_S n:
+  tiS n ⊈ n.
+Proof.
+  elim: n.
+  - inversion 1.
+  - move => ??. inversion 1; simplify_eq. naive_solver.
+  - move => ?? IH. inversion 1; simplify_K.
+    apply: IH. etrans; [|done]. econs. by econs.
+Qed.
+
+Lemma ti_lt_S n:
+  n ⊂ tiS n.
+Proof. split; [apply: ti_le_S | apply: ti_not_le_S]. Qed.
+
+Lemma ti_le_lt_S n1 n2:
+  n1 ⊂ tiS n2 →
+  n1 ⊆ n2.
+Proof.
+  elim: n1 n2.
+  - move => ??. econs.
+  - move => ? IH ? [Hle ?]. inversion Hle; simplify_eq. admit.
+  - move => ?? IH ? [Hle Hnle]. inversion Hle; simplify_K. constructor => ?.
+    apply: IH. split; [naive_solver|]. move => ?. apply: Hnle. by econs.
+Admitted.
+
+Lemma ti_lt_le (n1 n2 n3 : trace_index):
+  n1 ⊂ n2 → n2 ⊆ n3 → n1 ⊂ n3.
+Proof. move => [Hle1 Hnle] Hle. split; [by etrans|]. move => ?. apply: Hnle. by etrans. Qed.
+
+Lemma ti_lt_wf : wf (⊂@{trace_index}).
+Proof.
+  have H : forall n a : trace_index, a ⊂ n -> Acc (⊂) a; last first.
+  { move => n. apply: (H (tiS n)). apply ti_lt_S. }
+  elim.
+  - move => a [? Hnot]. contradict Hnot. econs.
+  - move => n IH a Hs. constructor => ??. apply: IH. apply: ti_lt_le; [done|]. by apply ti_le_lt_S.
+  - move => T f IH a [Hle Hnle].
+    (* inversion Hle; simplify_K. *)
+    (* + admit. *)
+    (* + admit. *)
+    (* + apply: IH. split; [done|]. contradict Hnle. constructor => ?. *)
+Admitted.
